still can't get bitvector lemma as stated by bryan to work

src/crypto/poly1305/x64/X64.Poly1305.Bitvectors_i.fst
@@ -10,53 +10,43 @@ open FStar.UInt.Base
 // tweak options?
 #reset-options "--smtencoding.elim_box true"
 
-
-
-
 val lemma_shr2: (x:uint_t 64) -> Lemma
   ((shift_right #64 x 2 == udiv #64 x 4))
-  // [SMTPat (shift_right #64 x 2)]
 let lemma_shr2 x = 
    assert_by_tactic (bv_tac()) (shift_right #64 x 2 == udiv #64 x 4)
 
 val lemma_shr4: x:uint_t 64 -> Lemma (shift_right #64 x 4 == udiv #64 x 16)
-				    // [SMTPat (shift_right #64 x 4)]
 let lemma_shr4 x =
   assert_by_tactic (bv_tac ()) (shift_right #64 x 4 == udiv #64 x 16)
 
 val lemma_and_mod_3: x:uint_t 64 -> Lemma (logand #64 x 3 == mod #64 x 4)
-				   // [SMTPat (logand #64 x 3)]
 let lemma_and_mod_3 x =
   assert_by_tactic (bv_tac ())
     (logand #64 x 3 == mod #64 x 4)
     
 val lemma_and_mod_15: x:uint_t 64 -> Lemma (logand #64 x 15 == mod #64 x 16)
-				   // [SMTPat (logand #64 x 15)]
 let lemma_and_mod_15 x =
   assert_by_tactic (bv_tac ()) 
     (logand #64 x 15 == mod #64 x 16)
 
 let lemma_clear_lower_2 x =
   assert_by_tactic (bv_tac ())
-  (logand #8 x 0xfc == mul_mod #8 (udiv #8 x 4) 4)
+  (logand #64 x 0xfffffffffffffffc == mul_mod #64 (udiv #64 x 4) 4)
 
 val lemma_and_0: x:uint_t 64 ->
   Lemma (logand #64 x 0 == 0)
-  // [SMTPat (logand #64 x 0)]
 let lemma_and_0 x =
   assert_by_tactic (bv_tac ())
   (logand #64 x 0 == (0 <: uint_t 64))
 
 val lemma_and_ones: x:uint_t 64 ->
   Lemma (logand #64 x 0xffffffffffffffff == x)
-  // [SMTPat (logand #64 x 0xffffffffffffffff)]
 let lemma_and_ones x =
    assert_by_tactic (bv_tac ())
      (logand #64 x 0xffffffffffffffff == x)
 
 val lemma_poly_constants_1: x:uint_t 64 -> 
   Lemma (logand #64 x 0x0ffffffc0fffffff < 0x1000000000000000)
-  // [SMTPat (logand #64 x 0x0ffffffc0fffffff)]
 let lemma_poly_constants_1 x =
   assert_by_tactic (bv_tac_lt 64)
     (logand #64 x 0x0ffffffc0fffffff < (0x1000000000000000 <: uint_t 64))
@@ -77,18 +67,17 @@ let lemma_poly_constants_3 x =
 
 val lemma_and_commutes: x:uint_t 64 -> y:uint_t 64 ->
   Lemma (logand #64 x y == logand #64 y x)
-  // [SMTPat (logand #64 x y == logand #64 y x)]
 let lemma_and_commutes x y =
   assert_by_tactic (bv_tac ())
     (logand #64 x y == logand #64 y x)
 
-// let lemma_bv128_64_64_and_helper x x0 x1 y y0 y1 z z0 z1 =
-//   admit ()
+let lemma_bv128_64_64_and_helper x x0 x1 y y0 y1 z z0 z1 =
+  admit ()
 
-// let bv128_64_64 x1 x0 = bvor (bvshl (bv_uext #64 #64 x1) 64) (bv_uext #64 #64 x0)
+let bv128_64_64 x1 x0 = bvor (bvshl (bv_uext #64 #64 x1) 64) (bv_uext #64 #64 x0)
 
-// let lemma_bv128_64_64_and x x0 x1 y y0 y1 z z0 z1 =
-//   admit ()
+let lemma_bv128_64_64_and x x0 x1 y y0 y1 z z0 z1 =
+  admit ()
 
 #reset-options "--smtencoding.elim_box true --z3cliopt smt.case_split=3"
 let lemma_bytes_shift_constants0 x =
@@ -223,22 +212,33 @@ let lemma_bytes_shift_power2 y =
   | _ -> ());
   lemma_bytes_power2 ()
 
-// let lowerUpper128 l u = l + (0x10000000000000000 * u)
-// let lemma_lowerUpper128_and x x0 x1 y y0 y1 z z0 z1 = admit ()
+let lowerUpper128 l u = l + (0x10000000000000000 * u)
+let lemma_lowerUpper128_and x x0 x1 y y0 y1 z z0 z1 = admit ()
 
-// open X64.Vale.Decls  // needed for shift_right64, logand64
-// open X64.Machine_s   // needed for mem
+open X64.Vale.Decls  // needed for shift_right64, logand64
+open X64.Machine_s   // needed for mem
+open FStar.Classical
+#reset-options "--smtencoding.elim_box true --smtencoding.nl_arith_repr native"
 
-// #reset-options "--smtencoding.elim_box true --smtencoding.nl_arith_repr native"
-
-// let lemma_poly_bits64 () =
-//   assert(forall (x:nat64). shift_right #64 x 2 == x / 4);
-//   assert(forall (x:nat64) (y:nat64). logand64 x y == logand #64 x y);
-//   assert(forall (x:nat64). logand #64 x 3 == mod #64 x 4);
-//   assert(forall (x:nat64). logand #64 x 15 == mod #64 x 16);
-//   assert(forall (x:nat64). logand #64 x 0 == 0);
-//   assert ((forall (x:nat64).	logand #64 x 0xffffffffffffffff == x));
-//   assert (forall (x:nat64). logand #64 x 0xfffffffffffffffc == (x / 4) * 4);
-//   assert (forall (x:nat64). logand #64 x 0x0ffffffc0fffffff < nat64_max / 16);
-//   assert (forall (x:nat64). logand #64 x 0x0ffffffc0ffffffc < nat64_max / 16);
-//   assert (forall (x:nat64). mod #64 (logand #64 x 0x0ffffffc0ffffffc) 4 == 0)
+let lemma_poly_bits64 () =
+  forall_intro (lemma_shr2);
+  assert(forall (x:nat64). shift_right #64 x 2 == udiv #64 x 4);
+  forall_intro (lemma_shr4);
+  assert(forall (x:nat64). shift_right #64 x 4 == udiv #64 x 16);
+  forall_intro (lemma_and_mod_3);
+  assert(forall (x:nat64). logand #64 x 3 == mod #64 x 4);
+  forall_intro (lemma_and_mod_15);
+  assert(forall (x:nat64). logand #64 x 15 == mod #64 x 16);
+  forall_intro (lemma_and_0);
+  assert(forall (x:nat64). logand #64 x 0 == 0);
+  forall_intro (lemma_and_ones);
+  assert ((forall (x:nat64).	logand #64 x 0xffffffffffffffff == x));
+  forall_intro (lemma_clear_lower_2);
+  assert (forall (x:nat64). logand #64 x 0xfffffffffffffffc == mul_mod #64 (udiv #64 x 4) 4);
+  forall_intro (lemma_poly_constants_1);
+  assert (forall (x:nat64). logand #64 x 0x0ffffffc0fffffff < nat64_max / 16);
+  forall_intro (lemma_poly_constants_2);
+  assert (forall (x:nat64). logand #64 x 0x0ffffffc0ffffffc < nat64_max / 16);
+  forall_intro (lemma_poly_constants_3);
+  assert (forall (x:nat64). mod #64 (logand #64 x 0x0ffffffc0ffffffc) 4 == 0);
+  assume(forall (x:nat64)  (y:nat64) . (logand64 x y) == (logand64 y x))
