src/crypto/poly1305/x64/X64.Poly1305.Bitvectors_i.fsti
@@ -6,32 +6,32 @@ open FStar.UInt.Vectors
 open FStar.UInt.Types
 open FStar.UInt.Base
 				    
-val lemma_clear_lower_2: x:uint_t 8 -> 
-  Lemma (logand #8 x 0xfc == mul_mod #8 (udiv #8 x 4) 4)
-  // [SMTPat (logand #8 x 0xfc)]
-// val lemma_bv128_64_64_and_helper: x:bv_t 128 -> x0:bv_t 64 -> x1:bv_t 64 ->
-//   y:bv_t 128 -> y0:bv_t 64 -> y1:bv_t 64 ->
-//   z:bv_t 128 -> z0:bv_t 64 -> z1:bv_t 64 ->
-//   Lemma (requires (z0 == bvand #64 x0 y0 /\
-// 		   z1 == bvand #64 x1 y1 /\
-// 		   x == bvor #128 (bvshl #128 (bv_uext #64 #64 x1) 64) 
-// 							   (bv_uext #64 #64 x0) /\
-// 		   y == bvor #128 (bvshl #128 (bv_uext #64 #64 y1) 64) 
-// 							   (bv_uext #64 #64 y0) /\
-// 		   z == bvor #128 (bvshl #128 (bv_uext #64 #64 z1) 64) 
-// 							   (bv_uext #64 #64 z0)))
-// 	(ensures (z == bvand #128 x y))
-// val bv128_64_64: x1:bv_t 64 -> x0:bv_t 64 -> Tot (bv_t 128)
+val lemma_clear_lower_2: x:uint_t 64 -> 
+  Lemma (logand #64 x 0xfffffffffffffffc == mul_mod #64 (udiv #64 x 4) 4)
 
-// val lemma_bv128_64_64_and: x:bv_t 128 -> x0:bv_t 64 -> x1:bv_t 64 ->
-//   y:bv_t 128 -> y0:bv_t 64 -> y1:bv_t 64 ->
-//   z:bv_t 128 -> z0:bv_t 64 -> z1:bv_t 64 ->
-//   Lemma (requires (z0 == bvand #64 x0 y0 /\
-// 		   z1 == bvand #64 x1 y1 /\
-// 		   x == bv128_64_64 x1 x0 /\
-// 		   y == bv128_64_64 y1 y0 /\
-// 		   z == bv128_64_64 z1 z0))
-// 	(ensures (z == bvand #128 x y))
+val lemma_bv128_64_64_and_helper: x:bv_t 128 -> x0:bv_t 64 -> x1:bv_t 64 ->
+  y:bv_t 128 -> y0:bv_t 64 -> y1:bv_t 64 ->
+  z:bv_t 128 -> z0:bv_t 64 -> z1:bv_t 64 ->
+  Lemma (requires (z0 == bvand #64 x0 y0 /\
+		   z1 == bvand #64 x1 y1 /\
+		   x == bvor #128 (bvshl #128 (bv_uext #64 #64 x1) 64) 
+							   (bv_uext #64 #64 x0) /\
+		   y == bvor #128 (bvshl #128 (bv_uext #64 #64 y1) 64) 
+							   (bv_uext #64 #64 y0) /\
+		   z == bvor #128 (bvshl #128 (bv_uext #64 #64 z1) 64) 
+							   (bv_uext #64 #64 z0)))
+	(ensures (z == bvand #128 x y))
+val bv128_64_64: x1:bv_t 64 -> x0:bv_t 64 -> Tot (bv_t 128)
+
+val lemma_bv128_64_64_and: x:bv_t 128 -> x0:bv_t 64 -> x1:bv_t 64 ->
+  y:bv_t 128 -> y0:bv_t 64 -> y1:bv_t 64 ->
+  z:bv_t 128 -> z0:bv_t 64 -> z1:bv_t 64 ->
+  Lemma (requires (z0 == bvand #64 x0 y0 /\
+		   z1 == bvand #64 x1 y1 /\
+		   x == bv128_64_64 x1 x0 /\
+		   y == bv128_64_64 y1 y0 /\
+		   z == bv128_64_64 z1 z0))
+	(ensures (z == bvand #128 x y))
 
 val lemma_bytes_shift_constants0: unit -> Lemma
     (shift_left #64 0 3 == 0 /\
@@ -99,13 +99,13 @@ Lemma (ensures (pow2 0 == 0x1 /\
 		pow2 48 == 0x1000000000000 /\
 		pow2 56 == 0x100000000000000))
 
-// val lemma_bytes_shift_power2: y:uint_t 64 ->
-//   Lemma (requires (y < 8))
-// 	(ensures  (shift_left #64 y 3 < 64 /\
-// 		   y * 8 == shift_left #64 y 3 /\
-// 		   pow2 (shift_left #64 y 3) == shift_left #64 1 (shift_left #64 y 3)))
+val lemma_bytes_shift_power2: y:uint_t 64 ->
+  Lemma (requires (y < 8))
+	(ensures  (shift_left #64 y 3 < 64 /\
+		   y * 8 == shift_left #64 y 3 /\
+		   pow2 (shift_left #64 y 3) == shift_left #64 1 (shift_left #64 y 3)))
 
-// val lowerUpper128: l:uint_t 64 -> u:uint_t 64 -> Tot (uint_t 128)
+val lowerUpper128: l:uint_t 64 -> u:uint_t 64 -> Tot (uint_t 128)
 
 // val lemma_lowerUpper128_and: x:uint_t 128 -> x0:uint_t 64 -> x1:uint_t 64 ->
 //   y:uint_t 128 -> y0:uint_t 64 -> y1:uint_t 64 ->
@@ -117,20 +117,20 @@ Lemma (ensures (pow2 0 == 0x1 /\
 // 		   z == lowerUpper128 z1 z0))
 // 	(ensures (z == logand #128 x y))
 
-// open X64.Vale.Decls  // needed for shift_right64, logand64
-// open X64.Machine_s   // needed for mem
-// val lemma_poly_bits64 : u:unit -> Lemma
-//   (requires True)
-//   (ensures
-//     (forall (x:nat64) . {:pattern (shift_right64 x 2)} shift_right64 x 2 == x / 4) /\
-//     (forall (x:nat64) . {:pattern (shift_right64 x 4)} shift_right64 x 4 == x / 16) /\
-//     (forall (x:nat64) . {:pattern (logand64 x 3)} logand64 x 3 == mod #64 x 4) /\
-//     (forall (x:nat64) . {:pattern (logand64 x 15)} logand64 x 15 == mod #64 x 16) /\
-//     (forall (x:nat64) . {:pattern (logand64 x 0)} logand64 x 0 == 0) /\
-//     (forall (x:nat64) . {:pattern (logand64 x 0xffffffffffffffff)} logand64 x 0xffffffffffffffff == x) /\
-//     (forall (x:nat64) . {:pattern (logand64 x 0xfffffffffffffffc)} logand64 x 0xfffffffffffffffc == (x / 4) * 4) /\
-//     (forall (x:nat64) . {:pattern (logand64 x 0x0ffffffc0fffffff)} logand64 x 0x0ffffffc0fffffff < nat64_max / 16) /\
-//     (forall (x:nat64) . {:pattern (logand64 x 0x0ffffffc0ffffffc)} logand64 x 0x0ffffffc0ffffffc < nat64_max / 16) /\
-//     (forall (x:nat64) . {:pattern (logand64 x 0x0ffffffc0ffffffc)} 
-// 		   mod #64 (logand64 x 0x0ffffffc0ffffffc) 4 == 0) /\
-//     (forall (x:nat64)  (y:nat64) . (logand64 x y) == (logand64 y x)))
+open X64.Vale.Decls  // needed for shift_right64, logand64
+open X64.Machine_s   // needed for mem
+val lemma_poly_bits64 : u:unit -> Lemma
+  (requires True)
+  (ensures
+    (forall (x:nat64) . {:pattern (shift_right64 x 2)} shift_right64 x 2 == x / 4) /\
+    (forall (x:nat64) . {:pattern (shift_right64 x 4)} shift_right64 x 4 == x / 16) /\
+    (forall (x:nat64) . {:pattern (logand64 x 3)} logand64 x 3 == x % 4) /\
+    (forall (x:nat64) . {:pattern (logand64 x 15)} logand64 x 15 == x % 16) /\
+    (forall (x:nat64) . {:pattern (logand64 x 0)} logand64 x 0 == 0) /\
+    (forall (x:nat64) . {:pattern (logand64 x 0xffffffffffffffff)} logand64 x 0xffffffffffffffff == x) /\
+    (forall (x:nat64) . {:pattern (logand64 x 0xfffffffffffffffc)} logand64 x 0xfffffffffffffffc == (x / 4) * 4) /\
+    (forall (x:nat64) . {:pattern (logand64 x 0x0ffffffc0fffffff)} logand64 x 0x0ffffffc0fffffff < nat64_max / 16) /\
+    (forall (x:nat64) . {:pattern (logand64 x 0x0ffffffc0ffffffc)} logand64 x 0x0ffffffc0ffffffc < nat64_max / 16) /\
+    (forall (x:nat64) . {:pattern (logand64 x 0x0ffffffc0ffffffc)} 
+		   mod #64 (logand64 x 0x0ffffffc0ffffffc) 4 == 0) /\
+    (forall (x:nat64)  (y:nat64) . (logand64 x y) == (logand64 y x)))
